Now that I've modified the experimental kernel to use strings rather than big ML expressions to build terms, the more_statements kluge can be done away with, at least for the moment.

holsrcs/statementsScript.sml
@@ -161,6 +161,117 @@ val _ = Hol_datatype`
 *)
 
 
+(* derived loop forms *)
+val forloop_def = Define`
+  forloop e1 e2 e3 bdy =
+       Block F []
+             [Standalone (NormE e1 base_se);
+              Trap BreakTrap
+                   (CLoop e2 (Block F [] [Trap ContTrap bdy;
+                                          Standalone (NormE e3 base_se)]))]
+`
+val whileloop_def = Define`
+  whileloop g s = Trap BreakTrap (CLoop (NormE g base_se) (Trap ContTrap s))
+`;
+val doloop_def = Define`
+  doloop bdy g =
+       Trap BreakTrap
+            (Block F [] [Trap ContTrap bdy;
+                         CLoop (NormE g base_se) (Trap ContTrap bdy)])
+`
+
+(* recursively check a predicate over a statement *)
+val rec_stmt_P_def = Define `
+  (rec_stmt_P (CLoop g bdy) =
+    \P. P (CLoop g bdy) /\ rec_stmt_P bdy P) /\
+  (rec_stmt_P (CIf g t f) =
+    \P. P (CIf g t f) /\ rec_stmt_P t P /\ rec_stmt_P f P) /\
+  (rec_stmt_P (Standalone e) = \P. P (Standalone e)) /\
+  (rec_stmt_P EmptyStmt = \P. P EmptyStmt) /\
+  (rec_stmt_P (Block b vds sts) =
+    \P. P (Block b vds sts) /\ rec_stmtl_P sts P) /\
+  (rec_stmt_P (Ret e) = \P. P (Ret e)) /\
+  (rec_stmt_P EmptyRet = \P. P EmptyRet) /\
+  (rec_stmt_P Break = \P. P Break) /\
+  (rec_stmt_P Cont = \P. P Cont) /\
+  (rec_stmt_P (Throw eopt) = \P. P (Throw eopt)) /\
+  (rec_stmt_P (Trap tt s) = \P. P (Trap tt s) /\ rec_stmt_P s P) /\
+  (rec_stmtl_P [] = \P. T) /\
+  (rec_stmtl_P (CONS x xs) = \P. rec_stmt_P x P /\ rec_stmtl_P xs P)
+`;
+val rec_stmtl_EVERY = store_thm(
+  "rec_stmtl_EVERY",
+  ``!stl P.
+        rec_stmtl_P stl P = EVERY (\st. rec_stmt_P st P) stl``,
+  Induct THEN ASM_SIMP_TAC (srw_ss()) [rec_stmt_P_def]);
+val _ = export_rewrites ["rec_stmtl_EVERY"]
+
+val erec_stmt_def = Define`
+  (erec_stmt P (CLoop g bdy) = erec_exte P g /\ erec_stmt P bdy) /\
+  (erec_stmt P (CIf g t f) =
+      erec_exte P g /\ erec_stmt P t /\ erec_stmt P f) /\
+  (erec_stmt P (Standalone ee) = erec_exte P ee) /\
+  (erec_stmt P EmptyStmt = T) /\
+  (erec_stmt P (Block b vds sts) = erec_vdecs P vds /\ erec_stmtl P sts) /\
+  (erec_stmt P (Ret ee) = erec_exte P ee) /\
+  (erec_stmt P EmptyRet = T) /\
+  (erec_stmt P Break = T) /\
+  (erec_stmt P Cont = T) /\
+  (erec_stmt P (Trap tt s) = erec_stmt P s) /\
+
+  (erec_stmtl P [] = T) /\
+  (erec_stmtl P (s::ss) = erec_stmt P s /\ erec_stmtl P ss) /\
+
+  (erec_exte P (NormE e se) = P e) /\
+  (erec_exte P (EStmt s c) = erec_stmt P s) /\
+
+  (erec_vdecs P [] = T) /\
+  (erec_vdecs P (vd::vds) = erec_vdec P vd /\ erec_vdecs P vds) /\
+
+  (erec_vdec P (VDec ty nm) = T) /\
+  (erec_vdec P (VDecInit ty nm i) = erec_idec P i) /\
+  (erec_vdec P (VDecInitA ty vloc i) = erec_idec P i) /\
+  (erec_vdec P (VStrDec cnm copt) = T) /\
+
+  (erec_idec P (DirectInit ee) = erec_exte P ee) /\
+  (erec_idec P (CopyInit ee) = erec_exte P ee)
+`
+
+(* categorising some forms of statement *)
+val is_retstmt_def = Define`
+  is_retstmt s = (?e. s = Ret e) \/ (s = EmptyRet)
+`;
+val is_intstmt_def = Define`
+  is_intstmt s = is_retstmt s \/ (s = Cont) \/ (s = Break)
+`;
+val retfree_def = Define`
+  retfree stmt = rec_stmt_P stmt ($~ o is_retstmt)
+`;
+val breakfree_def = Define`
+  breakfree stmt = rec_stmt_P stmt (\s. ~(s = Break))
+`;
+val contfree = Define`
+  contfree stmt = rec_stmt_P stmt (\s. ~(s = Cont))
+`
+val intstmt_free_def = Define`
+  intstmt_free stmt = rec_stmt_P stmt ($~ o is_intstmt)
+`
+
+val exception_stmt_def = Define`
+  (exception_stmt (Throw exn) = ?e. exn = SOME e) /\
+  (exception_stmt s = F)
+`;
+
+(* external declarations can appear at the top level of a translation unit *)
+val _ = Hol_datatype`
+  ext_decl = FnDefn of CPP_Type => CPPname => (string # CPP_Type) list => CStmt
+           | Decl of var_decl
+           | ClassConDef of CPPname => (string # CPP_Type) list =>
+                            mem_initializer list =>
+                            CStmt
+           | ClassDestDef of CPPname => CStmt
+           | TemplateDef of (CPP_Type # string) list => ext_decl
+`;
 
 
 val _ = export_theory();
