holsrcs/dynamicsScript.sml
@@ -14,7 +14,6 @@ local open wordsTheory integer_wordTheory finite_mapTheory in end
 (* C++ ancestor theories  *)
 open typesTheory memoryTheory expressionsTheory staticsTheory class_infoTheory
 open aggregatesTheory declaration_dynamicsTheory
-open more_statementsTheory
 local
   open side_effectsTheory statesTheory operatorsTheory overloadingTheory
 in end
